clean CFG

CFG.thy
@@ -14,54 +14,54 @@ datatype 'a cfg =
   CFG (\<NN> : "'a list") (\<TT> : "'a list") (\<RR> : "'a rules") (\<SS> : "'a")
 
 definition disjunct_symbols :: "'a cfg \<Rightarrow> bool" where
-  "disjunct_symbols cfg \<longleftrightarrow> set (\<NN> cfg) \<inter> set (\<TT> cfg) = {}"
+  "disjunct_symbols cfg \<equiv> set (\<NN> cfg) \<inter> set (\<TT> cfg) = {}"
 
 definition valid_startsymbol :: "'a cfg \<Rightarrow> bool" where
-  "valid_startsymbol cfg \<longleftrightarrow> \<SS> cfg \<in> set (\<NN> cfg)"
+  "valid_startsymbol cfg \<equiv> \<SS> cfg \<in> set (\<NN> cfg)"
 
 definition valid_rules :: "'a cfg \<Rightarrow> bool" where
-  "valid_rules cfg \<longleftrightarrow> (\<forall>(N, \<alpha>) \<in> set (\<RR> cfg). N \<in> set (\<NN> cfg) \<and> (\<forall>s \<in> set \<alpha>. s \<in> set (\<NN> cfg) \<union> set (\<TT> cfg)))"
+  "valid_rules cfg \<equiv> \<forall>(N, \<alpha>) \<in> set (\<RR> cfg). N \<in> set (\<NN> cfg) \<and> (\<forall>s \<in> set \<alpha>. s \<in> set (\<NN> cfg) \<union> set (\<TT> cfg))"
 
 definition distinct_rules :: "'a cfg \<Rightarrow> bool" where
-  "distinct_rules cfg = distinct (\<RR> cfg)"
+  "distinct_rules cfg \<equiv> distinct (\<RR> cfg)"
 
 definition wf_cfg :: "'a cfg \<Rightarrow> bool" where
-  "wf_cfg cfg \<longleftrightarrow> disjunct_symbols cfg \<and> valid_startsymbol cfg \<and> valid_rules cfg \<and> distinct_rules cfg"
+  "wf_cfg cfg \<equiv> disjunct_symbols cfg \<and> valid_startsymbol cfg \<and> valid_rules cfg \<and> distinct_rules cfg"
 
 lemmas wf_cfg_defs = wf_cfg_def valid_rules_def valid_startsymbol_def disjunct_symbols_def distinct_rules_def
 
 definition is_terminal :: "'a cfg \<Rightarrow> 'a \<Rightarrow> bool" where
-  "is_terminal cfg s = (s \<in> set (\<TT> cfg))"
+  "is_terminal cfg s \<equiv> s \<in> set (\<TT> cfg)"
 
 definition is_nonterminal :: "'a cfg \<Rightarrow> 'a \<Rightarrow> bool" where
-  "is_nonterminal cfg s = (s \<in> set (\<NN> cfg))"
+  "is_nonterminal cfg s \<equiv> s \<in> set (\<NN> cfg)"
 
 definition is_symbol :: "'a cfg \<Rightarrow> 'a \<Rightarrow> bool" where
-  "is_symbol cfg s \<longleftrightarrow> is_terminal cfg s \<or> is_nonterminal cfg s"
+  "is_symbol cfg s \<equiv> is_terminal cfg s \<or> is_nonterminal cfg s"
 
 definition wf_sentence :: "'a cfg \<Rightarrow> 'a sentence \<Rightarrow> bool" where
-  "wf_sentence cfg s = (\<forall>x \<in> set s. is_symbol cfg x)"
+  "wf_sentence cfg s \<equiv> \<forall>x \<in> set s. is_symbol cfg x"
 
-lemma is_nonterminal_startsymbol: "wf_cfg cfg \<Longrightarrow> is_nonterminal cfg (\<SS> cfg)"
+lemma is_nonterminal_startsymbol:
+  "wf_cfg cfg \<Longrightarrow> is_nonterminal cfg (\<SS> cfg)"
   by (simp add: is_nonterminal_def wf_cfg_defs)
 
 definition is_word :: "'a cfg \<Rightarrow> 'a sentence \<Rightarrow> bool" where
   "is_word cfg s = (\<forall>x \<in> set s. is_terminal cfg x)"
-   
+
 definition derives1 :: "'a cfg \<Rightarrow> 'a sentence \<Rightarrow> 'a sentence \<Rightarrow> bool" where
-  "derives1 cfg u v = 
-     (\<exists> x y N \<alpha>. 
-          u = x @ [N] @ y
-        \<and> v = x @ \<alpha> @ y
-        \<and> (N, \<alpha>) \<in> set (\<RR> cfg))"  
+  "derives1 cfg u v \<equiv> \<exists> x y N \<alpha>. 
+    u = x @ [N] @ y \<and>
+    v = x @ \<alpha> @ y \<and>
+    (N, \<alpha>) \<in> set (\<RR> cfg)"  
 
 definition derivations1 :: "'a cfg \<Rightarrow> ('a sentence \<times> 'a sentence) set" where
-  "derivations1 cfg = { (u,v) | u v. derives1 cfg u v }"
+  "derivations1 cfg \<equiv> { (u,v) | u v. derives1 cfg u v }"
 
 definition derivations :: "'a cfg \<Rightarrow> ('a sentence \<times> 'a sentence) set" where 
-  "derivations cfg = (derivations1 cfg)^*"
+  "derivations cfg \<equiv> (derivations1 cfg)^*"
 
 definition derives :: "'a cfg \<Rightarrow> 'a sentence \<Rightarrow> 'a sentence \<Rightarrow> bool" where
-  "derives cfg u v = ((u, v) \<in> derivations cfg)"
+  "derives cfg u v \<equiv> ((u, v) \<in> derivations cfg)"
 
 end
